CAM/Determinism.v
@@ -1,8 +1,21 @@
 Require Import Lang.Syntax.
+Require Import Lang.Tactics.
 Require Import Lang.ContextProperties.
 Require Import CAM.Syntax.
 Require Import CAM.Semantics.
 Require Import General.Tactics.
+Require Import General.Definitions.
+
+Theorem cam_deterministic : 
+  forall (V : Set), deterministic (@cam_red V).
+Proof.
+  intros V s1 s2 s3 Hstep1 Hstep2.
+  inv Hstep1; inv Hstep2; auto.
+  - Handles_contra.
+  - Handles_contra.
+  - specialize (HandlesOpWith_deterministic _ _ _ _ HHandlesOp HHandlesOp0) as ?.
+    subst. reflexivity.
+Qed.
 
 Lemma op_handle_not_handles_red :
   forall (V : Set) (C : i_ctx V) C' h l v s,
@@ -10,9 +23,10 @@ Lemma op_handle_not_handles_red :
     ~HandlesOp h l ->
     s = ⟨ C, o_ctx_handle C' h, l, v ⟩ₒ.
 Proof.
-  intros. inv H.
-  - reflexivity.
-  - exfalso. apply H0. exists e_op. assumption.
+  intros.
+  eapply cam_deterministic.
+  - apply H.
+  - apply cam_red_op_handle1; auto.
 Qed.
 
 Lemma op_handle_handles_red :
@@ -22,11 +36,10 @@ Lemma op_handle_handles_red :
     s = ⟨esubst (esubst e_op (vshift v))
               (v_lam (e_handle (o_ctx_shift C' [v_var VZ]ₒ) (hshift h))), C⟩ₑ.
 Proof.
-  intros. inv H.
-  - exfalso. apply HNotHandlesOp. exists e_op. assumption.
-  - assert (H : e_op = e_op0).
-    { eapply HandlesOpWith_deterministic. eauto. }
-    rewrite H. reflexivity.
+  intros.
+  eapply cam_deterministic.
+  - apply H.
+  - apply cam_red_op_handle2; auto.
 Qed.
 
 Lemma expr_val_red :
