CAM/Diverges.v
@@ -1,0 +1,130 @@
+Require Import General.Definitions.
+Require Import General.Lemmas.
+Require Import General.Tactics.
+Require Import Lang.Syntax.
+Require Import Lang.Semantics.
+Require Import Lang.ContextProperties.
+Require Import Lang.Determinism.
+Require Import Lang.NormalForm.
+Require Import CAM.Syntax.
+Require Import CAM.Semantics.
+Require Import CAM.Determinism.
+
+Theorem not_nf_and_diverges_cam :
+  forall (V : Set) (s n : cam_state V), normal_form cam_red n ->
+    ~(s ==>* n /\ diverges cam_red s).
+Proof.
+  intros. apply not_nf_and_diverges.
+  - apply cam_deterministic.  
+  - assumption.
+Qed.
+
+Definition cam_diverges_rel {V : Set} (s : cam_state V) :=
+  (exists C e, s = ⟨e, C⟩ₑ /\ diverges red (C[e]ᵢ))
+  \/ (exists C1 C2 l v,
+       s = ⟨C1, C2, l, v⟩ₒ
+       /\ diverges red (C1[ C2 [e_do l v ]ₒ ]ᵢ)
+       /\ ~OctxHandlesOp C2 l).
+
+Hint Unfold cam_diverges_rel : core.
+
+Theorem lang_cam_diverges :
+  forall (V : Set) (e : expr V),
+    diverges red e -> diverges cam_red ⟨e, i_ctx_top⟩ₑ.
+Proof.
+  intros V e He.
+  apply diverges_coind with (R := cam_diverges_rel).
+  - intros s Hs. destruct Hs as [[C [e' [? ?]]] | [C1 [C2 [l [v [? [? ?]]]]]]]; subst.
+    + inversion H0. subst. destruct e'.
+      * apply plug_val_red in H as [[? [? [? ?]]] | [? [? [? ?]]]]; subst.
+        -- eauto 10.
+        -- eauto 10.
+      * apply plug_add_red in H as [? [? [? [? ?]]]]; subst. eauto 10.
+      * apply plug_app_red in H as [? [? ?]]; subst. eauto 10.
+      * eauto 10.
+      * eauto 12.
+      * eauto 10.
+    + inversion H0. subst. destruct C1.
+      * simpl in H. exfalso.
+        specialize (lang_nf_correct _ (C2 [e_do l v ]ₒ)) as Hnf.
+        apply Hnf; eauto.
+      * eauto 12.
+      * destruct (HandlesOp_dec h l) as [[? ?] | ?].
+        -- apply (plug_handle_do_red _ _ _ _ _ _ x _) in H; auto; subst.
+           eauto 12.
+        (* It should be automated. *)
+        -- eexists. split.
+           ++ eauto.
+           ++ right. eexists. eexists. eexists. eexists. split.
+              ** auto.
+              ** split.
+                 --- apply H0.
+                 --- simpl. apply not_and_or. auto.
+  - eauto 10.
+Qed.
+
+Definition lang_diverges_rel {V : Set} (e : expr V) :=
+  (exists C e', e = C[e']ᵢ /\ diverges cam_red (⟨e', C⟩ₑ))
+  \/ (exists C C' l v,
+       e = (C[ C' [e_do l v ]ₒ ]ᵢ)
+       /\ diverges cam_red (⟨C, C', l, v⟩ₒ)
+       /\ ~OctxHandlesOp C' l).
+
+Hint Unfold lang_diverges_rel : core.
+
+Lemma cam_lang_op_mode_diverges :
+  forall (V : Set) (C : i_ctx V) C' l v, diverges cam_red ⟨ C, C', l, v ⟩ₒ ->
+    ~OctxHandlesOp C' l -> exists (e' : expr V),
+    C [C' [e_do l v ]ₒ ]ᵢ --> e' /\ lang_diverges_rel e'.
+Proof.
+  intros. generalize dependent C'. induction C;
+  intros; inversion H; subst.
+  - inv H1.
+  - inv H1. apply IHC with (C' := o_ctx_let C' e2); auto.
+  - destruct (HandlesOp_dec h l) as [[? ?] | ?].
+    + specialize (op_handle_handles_red _ _ _ _ _ _ _ _ H1 H3) as ?. subst.
+       eexists. split.
+       * simpl. apply red_context. apply red_handle_do; eauto.
+       * eauto 10.
+    + specialize (op_handle_not_handles_red _ _ _ _ _ _ _ H1 H3) as ?. subst.
+       apply IHC with (C' := o_ctx_handle C' h); simpl; auto.
+Qed.
+
+Theorem cam_lang_diverges :
+  forall (V : Set) (e : expr V),
+  diverges cam_red ⟨e, i_ctx_top⟩ₑ -> diverges red e.
+Proof.
+  intros.
+  apply diverges_coind with (R := lang_diverges_rel).
+  - clear e H. intros.
+    destruct H as [[C [e [? ?]]] | [C [C' [l [v [He [Hdiv HCe]]]]]]]; subst.
+    + generalize dependent C. induction e; intros.
+      * inv H0. apply expr_val_red in H as [[C' [e2 [? ?]]] | [C' [h [? ?]]]]; subst.
+        -- eexists. split.
+           ++ simpl. apply red_context. apply red_let.
+           ++ eauto 10.
+        -- eexists. split.
+           ++ simpl. apply red_context. apply red_handle_ret.
+           ++ eauto 10.
+      * inv H0. inv H. eexists. split.
+        -- apply red_context. apply red_add.
+        -- eauto 10.
+      * inv H0. inv H. eexists. split.
+        -- apply red_context. apply red_app.
+        -- eauto 10.
+      * inv H0. inv H. apply IHe1 with (C := i_ctx_let C e2); auto.
+      * inv H0. inv H. change (e_do l v) with (o_ctx_hole [ e_do l v ]ₒ).
+        apply cam_lang_op_mode_diverges; auto.
+      * inv H0. inv H. apply IHe with (C := i_ctx_handle C h); auto.
+    + apply cam_lang_op_mode_diverges; auto.
+  - left. exists i_ctx_top. exists e. eauto.
+Qed.
+
+Theorem lang_iff_cam_diverges :
+  forall (V : Set) (e : expr V),
+    diverges red e <-> diverges cam_red ⟨e, i_ctx_top⟩ₑ.
+Proof.
+  intros. split.
+  - apply lang_cam_diverges.
+  - apply cam_lang_diverges.
+Qed.
