General/Definitions.v
@@ -1,0 +1,41 @@
+Require Import General.Tactics.
+Require Import Coq.Relations.Operators_Properties.
+Require Import Coq.Relations.Relation_Operators.
+
+Definition normal_form {A : Set} (R : A -> A -> Prop) (a : A) :=
+  ~exists a', R a a'.
+
+Definition deterministic {A : Set} (R : A -> A -> Prop) :=
+  forall (a1 a2 a3 : A), R a1 a2 -> R a1 a3 -> a2 = a3.
+
+CoInductive diverges {A : Set} (E : A -> A -> Prop) : A -> Prop :=
+  | diverges_step : forall a1 a2, E a1 a2 -> diverges E a2 -> diverges E a1.
+
+Section diverges_coind.
+  Variable A : Set.
+  Variable E : A -> A -> Prop.
+  Variable R : A -> Prop.
+  Hypothesis Step : forall a, R a -> exists a', E a a' /\ R a'.
+
+  Theorem diverges_coind : forall a, R a -> diverges E a.
+  Proof.
+    cofix lang_inf_coind.
+    intros. apply Step in H as [a' [Hstep Ha']].
+    eapply diverges_step.
+    - apply Hstep.
+    - apply lang_inf_coind. assumption.
+  Qed.
+End diverges_coind.
+
+Theorem not_nf_and_diverges :
+  forall (A : Set) (R : A -> A -> Prop),
+    deterministic R ->
+    forall (a n : A), normal_form R n ->
+    ~(clos_refl_trans_1n _ R a n /\ diverges R a).
+Proof.
+  intros. intros [multi Hdiv]. induction multi.
+  - inv Hdiv. eauto.
+  - apply IHmulti; auto. inv Hdiv.
+    specialize (H _ _ _ H1 H2) as ?. subst.
+    assumption.
+Qed.
