Lang/Diverges.v
@@ -1,0 +1,27 @@
+Require Import General.Definitions.
+Require Import Lang.Syntax.
+Require Import Lang.Semantics.
+Require Import Lang.Determinism.
+
+Theorem not_nf_and_diverges_lang :
+  forall (V : Set) (e n : expr V), normal_form red n ->
+    ~(e -->* n /\ diverges red e).
+Proof.
+  intros. apply not_nf_and_diverges.
+  - apply lang_deterministic.  
+  - assumption.
+Qed.
+
+Definition ω := (v_lam (e_app (v_var VZ) (v_var VZ))) : value Empty_set.
+Definition Ω := e_app ω ω : expr Empty_set.
+
+Lemma omega_diverges :
+  diverges red Ω.
+Proof.
+  apply diverges_coind with (R := (fun e => e = Ω)).
+  - intros. subst. exists Ω. intuition.
+    assert (H : Ω = esubst (e_app (v_var VZ) (v_var VZ)) ω).
+    { unfold esubst. simpl. reflexivity. }
+    rewrite H at 2. apply red_app.
+  - reflexivity.
+Qed.
