Lang/Tactics.v
@@ -1,0 +1,7 @@
+Require Import Lang.Syntax.
+
+Ltac Handles_contra :=
+  match goal with
+  | [ H1 : ~HandlesOp ?h ?l, H2 : HandlesOpWith ?h ?l ?e  |- _ ] =>
+      exfalso; apply H1; exists e; apply H2
+  end.
